examples/bw/BW0.v
@@ -45,7 +45,7 @@ def flip(): Unit
     fun _ =>
       n <- trigger (PGet);; `n: Z <- n↓?;;
       let n := (n+1)%Z in
-      trigger (PPut n↑);;
+      trigger (PPut n↑);;;
       Ret Vundef
     .
 
