theories/ImpProofs.v
@@ -66,14 +66,14 @@ Section PROOFS.
         ge le0 x e
     :
       interp_imp ge le0 (denote_stmt (Assign x e)) =
-      interp_imp ge le0 (v <- denote_expr e ;; trigger (SetVar x v) ;; Ret Vundef).
+      interp_imp ge le0 (v <- denote_expr e ;; trigger (SetVar x v) ;;; Ret Vundef).
   Proof. reflexivity. Qed.
 
   Lemma denote_stmt_Seq
         ge le0 a b
     :
       interp_imp ge le0 (denote_stmt (Seq a b)) =
-      interp_imp ge le0 (denote_stmt a ;; denote_stmt b).
+      interp_imp ge le0 (denote_stmt a ;;; denote_stmt b).
   Proof. reflexivity. Qed.
 
   Lemma denote_stmt_If
@@ -102,7 +102,7 @@ Section PROOFS.
         ge le0 x X
     :
       interp_imp ge le0 (denote_stmt (AddrOf x X)) =
-      interp_imp ge le0 (v <- trigger (GetPtr X);; trigger (SetVar x v);; Ret Vundef).
+      interp_imp ge le0 (v <- trigger (GetPtr X);; trigger (SetVar x v);;; Ret Vundef).
   Proof. reflexivity. Qed.
 
   Lemma denote_stmt_Load
@@ -111,7 +111,7 @@ Section PROOFS.
       interp_imp ge le0 (denote_stmt (Load x pe)) =
       interp_imp ge le0 (p <- denote_expr pe;;
       v <- trigger (Call "load" (p↑));; v <- unwrapN(v↓);;
-      trigger (SetVar x v);; Ret Vundef).
+      trigger (SetVar x v);;; Ret Vundef).
   Proof. reflexivity. Qed.
 
   Lemma denote_stmt_Store
@@ -119,7 +119,7 @@ Section PROOFS.
     :
       interp_imp ge le0 (denote_stmt (Store pe ve)) =
       interp_imp ge le0 (p <- denote_expr pe;; v <- denote_expr ve;;
-      trigger (Call "store" ([p ; v]↑));; Ret Vundef).
+      trigger (Call "store" ([p ; v]↑));;; Ret Vundef).
   Proof. reflexivity. Qed.
 
   Lemma denote_stmt_Cmp
@@ -128,7 +128,7 @@ Section PROOFS.
       interp_imp ge le0 (denote_stmt (Cmp x ae be)) =
       interp_imp ge le0 ( a <- denote_expr ae;; b <- denote_expr be;;
       v <- trigger (Call "cmp" ([a ; b]↑));; v <- unwrapN (v↓);;
-      trigger (SetVar x v);; Ret Vundef).
+      trigger (SetVar x v);;; Ret Vundef).
   Proof. reflexivity. Qed.
 
   Lemma denote_stmt_CallFun1
@@ -141,7 +141,7 @@ Section PROOFS.
       else
         eval_args <- (denote_exprs args []);;
         v <- trigger (Call f (eval_args↑));; v <- unwrapN (v↓);;
-        trigger (SetVar x v);; Ret Vundef).
+        trigger (SetVar x v);;; Ret Vundef).
   Proof. reflexivity. Qed.
 
   Lemma denote_stmt_CallFun2
@@ -153,7 +153,7 @@ Section PROOFS.
       then triggerUB
       else
         eval_args <- (denote_exprs args []);;
-        trigger (Call f (eval_args↑));; Ret Vundef).
+        trigger (Call f (eval_args↑));;; Ret Vundef).
   Proof. reflexivity. Qed.
 
   Lemma denote_stmt_CallPtr1
@@ -167,7 +167,7 @@ Section PROOFS.
       else
         eval_args <- (denote_exprs args []);;
         v <- trigger (Call f (eval_args↑));; v <- unwrapN (v↓);;
-        trigger (SetVar x v);; Ret Vundef).
+        trigger (SetVar x v);;; Ret Vundef).
   Proof. reflexivity. Qed.
 
   Lemma denote_stmt_CallPtr2
@@ -180,7 +180,7 @@ Section PROOFS.
       then triggerUB
       else
         eval_args <- (denote_exprs args []);;
-        trigger (Call f (eval_args↑));; Ret Vundef).
+        trigger (Call f (eval_args↑));;; Ret Vundef).
   Proof. reflexivity. Qed.
 
   Lemma denote_stmt_CallSys1
@@ -190,7 +190,7 @@ Section PROOFS.
       interp_imp ge le0 (
       eval_args <- (denote_exprs args []);;
       v <- trigger (Syscall f eval_args top1);;
-      trigger (SetVar x v);; Ret Vundef).
+      trigger (SetVar x v);;; Ret Vundef).
   Proof. reflexivity. Qed.
 
   Lemma denote_stmt_CallSys2
@@ -199,7 +199,7 @@ Section PROOFS.
       interp_imp ge le0 (denote_stmt (CallSys2 f args)) =
       interp_imp ge le0 (
       eval_args <- (denote_exprs args []);;
-      trigger (Syscall f eval_args top1);; Ret Vundef).
+      trigger (Syscall f eval_args top1);;; Ret Vundef).
   Proof. reflexivity. Qed.
 
   (* interp_imp *)
@@ -303,7 +303,7 @@ Section PROOFS.
   Lemma interp_imp_SetVar_Vundef
         ge le0 x v
     :
-      interp_imp ge le0 (trigger (SetVar x v) ;; Ret Vundef) =
+      interp_imp ge le0 (trigger (SetVar x v) ;;; Ret Vundef) =
       tau;; tau;; Ret (alist_add x v le0, Vundef).
   Proof.
     unfold interp_imp, interp_GlobEnv, interp_ImpState. grind.
@@ -313,8 +313,8 @@ Section PROOFS.
   Lemma interp_imp_Call_only
         ge le0 f args
     :
-      interp_imp ge le0 (trigger (Call f args);; Ret Vundef) =
-      trigger (Call f args);; tau;; tau;; Ret (le0, Vundef).
+      interp_imp ge le0 (trigger (Call f args);;; Ret Vundef) =
+      trigger (Call f args);;; tau;; tau;; Ret (le0, Vundef).
   Proof.
     unfold interp_imp, interp_GlobEnv, interp_ImpState. grind.
     unfold pure_state. rewrite interp_trigger. grind.
@@ -325,7 +325,7 @@ Section PROOFS.
     :
       interp_imp ge le0
                  (v <- trigger (Call f args);; v <- unwrapN (v↓);;
-                  trigger (SetVar x v);; Ret Vundef) =
+                  trigger (SetVar x v);;; Ret Vundef) =
       v <- trigger (Call f args);;
       tau;; tau;; v <- unwrapN (v↓);;
       tau;; tau;; Ret (alist_add x v le0, Vundef).
@@ -340,8 +340,8 @@ Section PROOFS.
   Lemma interp_imp_Syscall_only
         ge le0 f args
     :
-      interp_imp ge le0 (trigger (Syscall f args top1);; Ret Vundef) =
-      trigger (Syscall f args top1);; tau;; tau;; Ret (le0, Vundef).
+      interp_imp ge le0 (trigger (Syscall f args top1);;; Ret Vundef) =
+      trigger (Syscall f args top1);;; tau;; tau;; Ret (le0, Vundef).
   Proof.
     unfold interp_imp, interp_GlobEnv, interp_ImpState. grind.
     unfold pure_state. rewrite interp_trigger. grind.
@@ -352,7 +352,7 @@ Section PROOFS.
     :
       interp_imp ge le0
                  (v <- trigger (Syscall f args top1);;
-                  trigger (SetVar x v);; Ret Vundef) =
+                  trigger (SetVar x v);;; Ret Vundef) =
       v <- trigger (Syscall f args top1);;
       tau;; tau;; tau;; tau;;
       Ret (alist_add x v le0, Vundef).
@@ -516,7 +516,7 @@ Section PROOFS.
       interp_imp ge le0 (denote_stmt (Store pe ve)) =
       '(le1, p) <- interp_imp ge le0 (denote_expr pe);;
       '(le2, v) <- interp_imp ge le1 (denote_expr ve);;
-      trigger (Call "store" ([p ; v]↑));; tau;; tau;; Ret (le2, Vundef).
+      trigger (Call "store" ([p ; v]↑));;; tau;; tau;; Ret (le2, Vundef).
   Proof.
     rewrite denote_stmt_Store. rewrite interp_imp_bind.
     grind. rewrite interp_imp_bind. grind.
@@ -552,7 +552,7 @@ Section PROOFS.
       interp_imp ge le0 (
                    eval_args <- (denote_exprs args acc);;
                    v <- trigger (Call f (eval_args↑));; v <- unwrapN (v↓);;
-                   trigger (SetVar x v);; Ret Vundef)
+                   trigger (SetVar x v);;; Ret Vundef)
       =
       '(le1, vs) <- interp_imp_denote_exprs ge le0 args acc;;
       v <- trigger (Call f (vs↑));;
@@ -570,10 +570,10 @@ Section PROOFS.
     :
       interp_imp ge le0 (
                    eval_args <- (denote_exprs args acc);;
-                   trigger (Call f (eval_args↑));; Ret Vundef)
+                   trigger (Call f (eval_args↑));;; Ret Vundef)
       =
       '(le1, vs) <- interp_imp_denote_exprs ge le0 args acc;;
-      trigger (Call f (vs↑));;
+      trigger (Call f (vs↑));;;
       tau;; tau;; Ret (le1, Vundef).
   Proof.
     move args before Σ. revert_until args. induction args; i.
@@ -606,7 +606,7 @@ Section PROOFS.
       then triggerUB
       else
         '(le1, vs) <- interp_imp_denote_exprs ge le0 args [];;
-        trigger (Call f (vs↑));;
+        trigger (Call f (vs↑));;;
         tau;; tau;; Ret (le1, Vundef).
   Proof.
     rewrite denote_stmt_CallFun2. des_ifs; try (apply interp_imp_exprs_only).
@@ -659,7 +659,7 @@ Section PROOFS.
           else
             tau;;
             '(le2, vs) <- interp_imp_denote_exprs ge le1 args [];;
-            trigger (Call f (vs↑));;
+            trigger (Call f (vs↑));;;
             tau;; tau;; Ret (le2, Vundef)
         | None => triggerUB
         end
@@ -682,7 +682,7 @@ Section PROOFS.
       interp_imp ge le0 (
                    eval_args <- (denote_exprs args acc);;
                    v <- trigger (Syscall f eval_args top1);;
-                   trigger (SetVar x v);; Ret Vundef)
+                   trigger (SetVar x v);;; Ret Vundef)
       =
       '(le1, vs) <- interp_imp_denote_exprs ge le0 args acc;;
       v <- trigger (Syscall f vs top1);;
@@ -699,10 +699,10 @@ Section PROOFS.
     :
       interp_imp ge le0 (
                    eval_args <- (denote_exprs args acc);;
-                   trigger (Syscall f eval_args top1);; Ret Vundef)
+                   trigger (Syscall f eval_args top1);;; Ret Vundef)
       =
       '(le1, vs) <- interp_imp_denote_exprs ge le0 args acc;;
-      trigger (Syscall f vs top1);;
+      trigger (Syscall f vs top1);;;
       tau;; tau;; Ret (le1, Vundef).
   Proof.
     move args before Σ. revert_until args. induction args; i.
@@ -727,7 +727,7 @@ Section PROOFS.
     :
       interp_imp ge le0 (denote_stmt (CallSys2 f args)) =
       '(le1, vs) <- interp_imp_denote_exprs ge le0 args [];;
-      trigger (Syscall f vs top1);;
+      trigger (Syscall f vs top1);;;
       tau;; tau;;
       Ret (le1, Vundef).
   Proof.
